
### Reciprocal 

The reciprocal trigonometric identities are:

- $\sin \theta = \frac{1}{\csc \theta}$ 
- $\cos \theta = \frac{1}{\sec \theta}$
- $\tan \theta = \frac{1}{\cot \theta}$ 
- $\csc \theta = \frac{1}{\sin \theta}$ 
- $\sec \theta = \frac{1}{\cos \theta}$
- $\cot \theta = \frac{1}{\tan \theta}$ 

### Pythagorean 
There are three Pythagorean trigonometric identities in trigonometry that are based on the right-triangle theorem or Pythagoras theorem.

- $\sin^2 \theta + \cos^2 \theta = 1$
- $1+\tan^2 \theta = \sec^2 \theta$ 
- $\csc^2 \theta = 1 + \cot^2 \theta$ 

### Ratio
The trigonometric ratio identities are:

- $\tan \theta = \frac{\sin \theta}{\cos \theta}$ 
- $\cot \theta = \frac{\cos \theta}{\sin \theta}$

### Opposite Angles
The list of opposite angle trigonometric identities are:

- $\sin(-\theta) = -\sin \theta$ 
- $\cos(-\theta) = \cos \theta$ 
- $\tan(-\theta) = \tan \theta$ 
- $\cot(-\theta) = -\cot \theta$ 
- $\sec(-\theta) = \sec \theta$
- $\csc(-\theta) = -\csc \theta$ 


### Complementary Angles

In geometry, two angles are complementary if their sum is equal to 90 degrees. Similarly, when we can learn here the trigonometric identities for complementary angles.

-   $\sin (90 –\theta) = \cos\theta$
-   $\cos (90 –\theta) = \sin\theta$
-   $\tan (90 –\theta) = \cot\theta$
-   $\cot ( 90 –\theta) = \tan\theta$
-   $\sec (90 –\theta) = \csc\theta$
-   $\csc (90 –\theta) = \sec\theta$

### Supplementary Angles

> [!blank-container|right-medium]
> ![[supplementary_angles.svg]]


Two angles are supplementary if their sum is equal to 90 degrees. Similarly, when we can learn here the trigonometric identities for supplementary angles.


-   $\sin (180 –\theta) = \sin\theta$
-   $\cos (180 - \theta) = -\cos\theta$
-   $\tan (180-\theta) = -\tan\theta$
-   $\cot (180-\theta) = -\cot\theta$
-   $\sec (180-\theta) = -\sec\theta$
-   $\csc (180-\theta) = \csc\theta$


### Sum and difference of angles
- $\cos(\alpha+\beta)=\cos\alpha\cos\beta–\sin\alpha\sin\beta$
- $\cos(\alpha-\beta)=\cos\alpha\cos\beta+\sin\alpha\sin\beta$
- $\sin(\alpha+\beta)=\sin\alpha\cos\beta+\cos\alpha\sin\beta$
- $\sin(\alpha-\beta)=\sin\alpha\cos\beta-\cos\alpha\sin\beta$
- $\tan(\alpha+\beta)=\frac{\tan \alpha + \tan \beta}{1-\tan\alpha\tan\beta}$
- $\tan(\alpha-\beta)=\frac{\tan \alpha - \tan \beta}{1+\tan\alpha\tan\beta}$


### Double Angle
If the angles are doubled, then the trigonometric identities for sin, cos and tan are:

- $\sin (2\theta) = 2 \sin\theta\cos\theta$  
- $\cos (2\theta) = \cos^2\theta-\sin^2\theta=2\cos^2\theta-1=1-2\sin^2\theta$ 
- $\tan(2\theta)=\frac{2\tan\theta}{1-\tan^2\theta}$ 

### Half Angle 
If the angles are halved, then the trigonometric identities for sin, cos and tan are:

- $\sin\frac{\theta}{2} = \pm \sqrt{\frac{1-\cos\theta}{2}}$ 
- $\cos\frac{\theta}{2} = \pm \sqrt{\frac{1+\cos\theta}{2}}$ 
- $\tan\frac{\theta}{2} = \pm \sqrt{\frac{1-\cos\theta}{1+\cos\theta}}$ 

### Product-Sum
The product-sum trigonometric identities change the sum or difference of sines or cosines into a product of sines and cosines. 

- $\sin \theta + \sin \phi = 2 \sin \left( \frac{\theta+\phi}{2} \right)\cos \left( \frac{\theta-\phi}{2} \right)$ 
- $\cos \theta + \cos \phi = 2 \cos \left( \frac{\theta+\phi}{2} \right)\cos \left( \frac{\theta-\phi}{2} \right)$  
- $\sin \theta - \sin \phi = 2 \cos \left( \frac{\theta+\phi}{2} \right)\sin \left( \frac{\theta-\phi}{2} \right)$ 
- $\cos \theta - \cos \phi = -2 \sin \left( \frac{\theta+\phi}{2} \right)\sin \left( \frac{\theta-\phi}{2} \right)$ 

### Products

- $\sin \theta \sin \phi = \left[\cos (\theta - \phi) - \cos(\theta + \phi)\right]/2$ 
- $\sin \theta \cos \phi = \left[\sin (\theta + \phi) - \sin(\theta - \phi)\right]/2$
- $\cos \theta \cos \phi = \left[\cos (\theta + \phi) - \cos(\theta - \phi)\right]/2$


### Identities


$$
\begin{align}
\cos (x)&=\sin\left(\frac \pi 2 - x\right) \\
\frac 1 {\cos (x)} &=\frac 1 {\sin\left(\frac \pi 2 - x\right)} \\
\operatorname{sec} (x) &=\operatorname{csc}\left(\frac \pi 2 - y\right) \\
\end{align}
$$





Sure, the identity arccsc(x) = arcsec(1/x) for x > 0 can be understood from the reciprocal relationship between the cosecant and secant functions.

The cosecant function csc(x) is defined as 1/sin(x), and the secant function sec(x) is defined as 1/cos(x). Furthermore, the identity sin(x) = cos(π/2 - x) holds true.

Therefore, for any x in the domain of these functions, we have:

$$1/sin(x) = 1/cos(\pi/2 - x)$$

Given that $\sec(y) = 1/\cos(y)$, and $\csc(y) = 1/\sin(y)$, the above relationship can be written as:

$$
\begin{align}
y=\csc(x) &= \sec(\pi/2 - x) \\
\operatorname{arccsc}(y)=x &= \operatorname{arccsc}\left(\sec\left(\frac \pi 2 - x\right)\right)
\end{align}
$$

Therefore, if we take $y = \csc(x)$, which implies that $x = arccsc(y)$, then from the above relationship we get:

arccsc(y) = π/2 - sec^(-1)(y), which simplifies to:

arccsc(y) = sec^(-1)(1/y) when y is positive, because 1/sec(x) = cos(x), and cos(π/2 - θ) = sin(θ), which is always positive when θ is in (0, π/2).

Hence, arccsc(x) = arcsec(1/x) for x > 0.

This identity can be very useful when dealing with integrals, because it allows you to switch between the two forms based on which one is easier to handle in a given situation.

$$
\begin{align}
y&=\csc(x) \\
y&=\frac 1 {\sin(x)} \\
\frac 1 y&=\sin(x) \\
\operatorname{arcsin}\left(\frac 1 y\right)&=x \\
\end{align}
$$




$$
\begin{align}
y=\sin(x) &= \cos\left(\frac \pi 2 - x\right) \\
\operatorname{arccos}(y) &= \frac \pi 2 - x \\
\operatorname{arccos}(\sin(x)) &= \frac \pi 2 - x \\
x &= \frac \pi 2 - \operatorname{arccos}(y) \\
\operatorname{arcsin}(y) &= \frac \pi 2 - \operatorname{arccos}(y) \\
\end{align}
$$


$$
\begin{align}
y=\csc(x) &= \sec\left(\frac \pi 2 - x\right) \\
\operatorname{arcsec}(y) &= \frac \pi 2 - x \\
\operatorname{arcsec}(\csc(x)) &= \frac \pi 2 - x \\
x &= \frac \pi 2 - \operatorname{arcsec}(y) \\
\operatorname{arccsc}(y) &= \frac \pi 2 - \operatorname{arcsec}(y) \\
\end{align}
$$

$$
\begin{align}
\frac 1 y=\sin(x) &= \cos\left(\frac \pi 2 - x\right) \\
y=\csc(x)&, \quad \operatorname{arccsc}(y) = x \\
\operatorname{arccos}\left(\frac 1 y\right) &= \frac \pi 2 - x \\
\operatorname{arccos}(\sin(x)) &= \frac \pi 2 - x \\
x &= \frac \pi 2 - \operatorname{arccos}\left(\frac 1 y\right) \\
\operatorname{arccsc}(y) &= \frac \pi 2 - \operatorname{arccos}\left(\frac 1 y\right) \\
\operatorname{arcsin}\left(\frac 1 y\right) &= \frac \pi 2 - \operatorname{arccos}\left(\frac 1 y\right) \\
\end{align}
$$

---

$$
\begin{array}{ll}
\sin\left(\operatorname{arcsec}(x)\right) &= \frac{\sqrt{x^2-1}}{x} \\
\cos\left(\operatorname{arcsec}(x)\right) &= \frac{1}{x} \\
\operatorname{arccosh}(x) &= \log(x+\sqrt{x-1}\sqrt{x+1})
\end{array}
$$
### Inverse Trigonometric Identities

$$
\begin{array}{ll}
&\arcsin(-x) &=-\arcsin x&, |x| \leq 1 \\
&\arccos(-x) &=\pi-\arccos x&, |x| \leq 1 \\
&\arctan(-x) &=-\arctan x&,  x \in \mathbb{R} \\
&\operatorname{arccot}(-x) &=\pi-\operatorname{arccot} x&,  x \in \mathbb{R} \\
&\operatorname{arccsc} x &=\arcsin\left(\frac{1}{x}\right)&, |x| \geq 1 \\
&\operatorname{arcsec} x &=\arccos\left(\frac{1}{x}\right)&, |x| \geq 1 \\
&\operatorname{arccot} x &=\arctan\left(\frac{1}{x}\right)&,  x>0 \\
&\operatorname{arccot} x &=\pi+\arctan\left(\frac{1}{x}\right)&,  x<0 \\
&\arcsin x+\arccos x&=\frac{\pi}{2}&, |x| \leq 1 \\
&\operatorname{arccsc} x+\operatorname{arcsec} x&=\frac{\pi}{2}&, |x| \geq 1 \\
&\arcsin x &=\arccos\left(\sqrt{1-x^2}\right)&,  x \geq 0 \\
&\arccos x &=\arcsin\left(\sqrt{1-x^2}\right)&,  x \geq 0 \\
&\arccos x &=\pi-\arcsin\left(\sqrt{1-x^2}\right)&,  x<0 \\
&\arctan x+\arctan y&=\arctan\left(\frac{x+y}{1-x y}\right)&,  x y<1 \\
&\arctan x+\arctan y&=\pi+\arctan\left(\frac{x+y}{1-x y}\right)&,  x y>1 \\
&\arctan x-\arctan y&=\arctan\left(\frac{x-y}{1+x y}\right) \\
&\arcsin x &=\arctan\left(\frac{x}{\sqrt{1-x^2}}\right)&,  x \in(0&,1) \\
&\arccos x &=\arctan\left(\frac{\sqrt{1-x^2}}{x}\right)&,  x \in(0&,1) \\
&\arctan x &=\arcsin\left(\frac{x}{\sqrt{x^2+1}}\right)&,  x>0 \\
&\arctan x &=\arccos\left(\frac{1}{\sqrt{x^2+1}}\right)&,  x>0 \\
&
\end{array}
$$

